Finish semax_return in canonical form. Finish new forward_return tactic. Ready to test.

floyd/canon.v
@@ -2120,20 +2120,58 @@ Proof.
     apply make_args0_tc_environ; auto.
 Qed.
 
-Lemma semax_return_None: forall {cs Espec} Delta Ppre Qpre Rpre Ppost Rpost,
+Inductive return_outer_gen: ret_assert -> ret_assert -> Prop :=
+| return_outer_gen_refl: forall P t,
+    return_outer_gen
+      (frame_ret_assert (function_body_ret_assert t P) emp)
+      (frame_ret_assert (function_body_ret_assert t P) emp)
+| return_outer_gen_switch: forall P Q,
+    return_outer_gen P Q ->
+    return_outer_gen (switch_ret_assert P) Q
+| return_outer_gen_post: forall post P Q,
+    return_outer_gen P Q ->
+    return_outer_gen (overridePost post P) Q
+| return_outer_gen_loop1: forall inv P Q,
+    return_outer_gen P Q ->
+    return_outer_gen (loop1_ret_assert inv P) Q
+| return_outer_gen_loop2: forall inv P Q,
+    return_outer_gen P Q ->
+    return_outer_gen (loop2_ret_assert inv P) Q.
+
+Lemma return_outer_gen_spec: forall P Q,
+  return_outer_gen P Q ->
+  P EK_return = Q EK_return.
+Proof.
+  intros.
+  induction H.
+  + auto.
+  + etransitivity; [| eassumption].
+    auto.
+  + etransitivity; [| eassumption].
+    auto.
+  + etransitivity; [| eassumption].
+    auto.
+  + etransitivity; [| eassumption].
+    auto.
+Qed.
+
+Lemma semax_return_None: forall {cs Espec} Delta Ppre Qpre Post Rpre Ppost Rpost,
   ret_type Delta = Tvoid ->
-  ENTAIL Delta, PROPx Ppre (LOCALx Qpre (SEPx Rpre)) |-- PROPx Ppost (LOCALx nil (SEPx Rpost)) ->  
-  @semax cs Espec Delta (PROPx Ppre (LOCALx Qpre (SEPx Rpre))) (Sreturn None)
-     (frame_ret_assert (function_body_ret_assert (ret_type Delta) (PROPx Ppost (LOCALx nil (SEPx Rpost)))) emp).
+  return_outer_gen Post
+    (frame_ret_assert (function_body_ret_assert (ret_type Delta) (PROPx Ppost (LOCALx nil (SEPx Rpost)))) emp) ->
+  ENTAIL Delta, PROPx Ppre (LOCALx Qpre (SEPx Rpre)) |-- PROPx Ppost (LOCALx nil (SEPx Rpost)) ->
+  @semax cs Espec Delta (PROPx Ppre (LOCALx Qpre (SEPx Rpre))) (Sreturn None) Post.
 Proof.
   intros.
   eapply semax_pre; [| apply semax_return].
+  apply return_outer_gen_spec in H0.
+  rewrite H0; clear Post H0.
   rewrite frame_ret_assert_emp.
   apply andp_right.
   + unfold tc_expropt.
     unfold_lift; intros rho; apply prop_right; auto.
   + unfold cast_expropt, id.
-    eapply derives_trans; [exact H0 |].
+    eapply derives_trans; [exact H1 |].
     unfold_lift.
     go_lowerx.
     rewrite H.
@@ -2141,15 +2179,28 @@ Proof.
 Qed.
 
 Inductive return_Some_post_gen (v_gen: val): (environ -> mpred) -> (environ -> mpred) -> Prop :=
+| return_Some_post_gen_main: forall P ts u,
+    return_Some_post_gen v_gen (main_post P ts u) `TT
 | return_Some_post_gen_canon:
     forall P v R,
       return_Some_post_gen v_gen
         (PROPx P (LOCALx (temp ret_temp v ::  nil) (SEPx R)))
         (PROPx (P ++ (v_gen = v) :: nil) (LOCALx nil (SEPx R)))
-| return_Some_post_gen_EX:
+| return_Some_post_gen_EX':
     forall (A: Type) (post1 post2: A -> environ -> mpred),
       (forall a: A, return_Some_post_gen v_gen (post1 a) (post2 a)) ->
       return_Some_post_gen v_gen (exp post1) (exp post2).
+
+Lemma return_Some_post_gen_EX: forall v_gen A post1 post2,
+  (forall a: A, exists P, return_Some_post_gen v_gen (post1 a) P /\ P = post2 a) ->
+  return_Some_post_gen v_gen (exp post1) (exp post2).
+Proof.
+  intros.
+  apply return_Some_post_gen_EX'.
+  intro a; specialize (H a).
+  destruct H as [? [? ?]]; subst.
+  auto.
+Qed.
 
 Lemma return_Some_post_gen_spec: forall v_gen post1 post2,
   return_Some_post_gen v_gen post1 post2 ->
@@ -2157,6 +2208,8 @@ Lemma return_Some_post_gen_spec: forall v_gen post1 post2,
 Proof.
   intros.
   induction H.
+  + unfold main_post.
+    intros rho; simpl; auto.
   + erewrite PROPx_Permutation by apply Permutation_app_comm.
     simpl app.
     go_lowerx.
@@ -2173,21 +2226,23 @@ Proof.
     apply (exp_right a); auto.
 Qed.
 
-Lemma semax_return_Some: forall {cs Espec} Delta Ppre Qpre Rpre post1 post2 ret v_gen,
+Lemma semax_return_Some: forall {cs Espec} Delta Ppre Qpre Rpre Post1 post2 post3 ret v_gen,
   ENTAIL Delta, PROPx Ppre (LOCALx Qpre (SEPx Rpre)) |-- local (`(eq v_gen) (eval_expr (Ecast ret (ret_type Delta)))) ->
   ENTAIL Delta, PROPx Ppre (LOCALx Qpre (SEPx Rpre)) |-- tc_expr Delta (Ecast ret (ret_type Delta)) ->
-  return_Some_post_gen v_gen post1 post2 ->
-  ENTAIL Delta, PROPx Ppre (LOCALx Qpre (SEPx Rpre)) |-- post2 ->  
-  @semax cs Espec Delta (PROPx Ppre (LOCALx Qpre (SEPx Rpre))) (Sreturn (Some ret))
-     (frame_ret_assert (function_body_ret_assert (ret_type Delta) post1) emp).
+  return_outer_gen Post1 (frame_ret_assert (function_body_ret_assert (ret_type Delta) post2) emp) ->
+  return_Some_post_gen v_gen post2 post3 ->
+  ENTAIL Delta, PROPx Ppre (LOCALx Qpre (SEPx Rpre)) |-- post3 ->
+  @semax cs Espec Delta (PROPx Ppre (LOCALx Qpre (SEPx Rpre))) (Sreturn (Some ret)) Post1.
 Proof.
   intros.
   eapply semax_pre; [| apply semax_return].
+  apply return_outer_gen_spec in H1.
+  rewrite H1; clear Post1 H1.
   apply andp_right; [exact H0 |].
   rewrite frame_ret_assert_emp.
   unfold cast_expropt.
   assert (ENTAIL Delta, PROPx Ppre (LOCALx Qpre (SEPx Rpre))
-            |-- ` (function_body_ret_assert (ret_type Delta) post1 EK_return (Some v_gen)) id).
+            |-- ` (function_body_ret_assert (ret_type Delta) post2 EK_return (Some v_gen)) id).
   + unfold function_body_ret_assert, bind_ret, id.
     unfold_lift.
     apply andp_right.
@@ -2198,9 +2253,9 @@ Proof.
       unfold_lift; normalize.
       eapply derives_trans; [apply typecheck_expr_sound; auto |].
       simpl. auto.
-    - apply (derives_trans _ _ _ H2).
+    - apply (derives_trans _ _ _ H3).
       apply return_Some_post_gen_spec; auto.
-  + rewrite (add_andp _ _ H3), (add_andp _ _ H).
+  + rewrite (add_andp _ _ H1), (add_andp _ _ H).
     rewrite (andp_comm _ (PROPx _ _)), !andp_assoc.
     apply andp_left2.
     go_lowerx.
